chore(na): Add MagicLTy(pe) + na token pass through

theories/rust_typing/ltypes.v
@@ -779,6 +779,11 @@ Section ltype_def.
         (κs : list lft)
         (lt_full : lty)
     | ShadowedLty {rt : Type} (lt_cur : lty) (r_cur : place_rfn rt) (lt_full : lty)
+    | MagicLty
+        {rt_full : Type}
+        (lt_cur : lty) (lt_full : lty)
+        (Cpre : coPset → rt_full → iProp Σ)
+        (Cpost : coPset → rt_full → iProp Σ)
   .
 
   (*
@@ -812,6 +817,8 @@ Section ltype_def.
         lty_rt lt_full
     | ShadowedLty lt_cur r_cur lt_full =>
         lty_rt lt_full
+    | MagicLty lt_cur _ _ _ =>
+        lty_rt lt_cur
     end.
 
   Fixpoint lty_st (lt : lty) : syn_type :=
@@ -832,6 +839,8 @@ Section ltype_def.
         lty_st lt_full
     | ShadowedLty lt_cur r_cur lt_full =>
         lty_st lt_full
+    | MagicLty lt_cur _ _ _ =>
+        lty_st lt_cur
     end.
 
   Fixpoint lty_wf (lt : lty) : Prop :=
@@ -857,6 +866,8 @@ Section ltype_def.
         lty_wf lt
     | @ShadowedLty rt_cur lt_cur r_cur lt_full =>
         lty_wf lt_cur ∧ lty_wf lt_full ∧ lty_rt lt_cur = rt_cur
+    | @MagicLty rt_full lt_cur lt_full _ _ =>
+        rt_full = lty_rt lt_full ∧ lty_wf lt_cur ∧ lty_wf lt_full
     end.
 
 
@@ -881,9 +892,12 @@ Section ltype_def.
           P lt_cur → P lt_inner → P lt_full → P (OpenedLty lt_cur lt_inner lt_full Cpre Cpost)) →
       (∀ κs (lt_full : lty), P lt_full → P (CoreableLty κs lt_full)) →
       (∀ (rt_cur : Type) (lt_cur : lty) (r_cur : place_rfn rt_cur) (lt_full : lty), P lt_cur → P lt_full → P (ShadowedLty lt_cur r_cur lt_full)) →
+      (∀ (rt_full : Type) (lt_cur lt_full : lty)
+        (Cpre : coPset → rt_full → iProp Σ) (Cpost : coPset → rt_full → iProp Σ),
+          P lt_cur → P lt_full → P (MagicLty lt_cur lt_full Cpre Cpost)) →
       ∀ lt : lty, P lt.
   Proof.
-    intros P Hblocked Hshrblocked Hofty Halias Hmut Hshr Hbox Hptr Hstruct Harr Henum Hopened Hcoreable Hshadow.
+    intros P Hblocked Hshrblocked Hofty Halias Hmut Hshr Hbox Hptr Hstruct Harr Henum Hopened Hcoreable Hshadow Hmagic.
     (* doing induction does not give us the IH *)
     refine (fix IH (lt : lty) {struct lt} : P lt :=
       match lt return (P lt) with
@@ -907,7 +921,9 @@ Section ltype_def.
           _
       | ShadowedLty lt_cur r_cur lt_full =>
           _
-      end); [apply IH.. | | | | | | ].
+      | MagicLty _ _ _ _ =>
+          _
+      end); [apply IH.. | | | | | | | ].
       - apply Hstruct.
         apply list_is_list_full.
         apply IH.
@@ -916,6 +932,7 @@ Section ltype_def.
       - apply Hopened; apply IH.
       - apply Hcoreable; apply IH.
       - apply Hshadow; apply IH.
+      - apply Hmagic; apply IH.
   Defined.
 
   Lemma lty_induction :
@@ -936,10 +953,13 @@ Section ltype_def.
           P lt_cur → P lt_inner → P lt_full → P (OpenedLty lt_cur lt_inner lt_full Cpre Cpost)) →
       (∀ κs (lt_full : lty), P lt_full → P (CoreableLty κs lt_full)) →
       (∀ (rt_cur : Type) (lt_cur : lty) (r_cur : place_rfn rt_cur) (lt_full : lty), P lt_cur → P lt_full → P (ShadowedLty lt_cur r_cur lt_full)) →
+      (∀ (rt_full : Type) (lt_cur lt_full : lty)
+        (Cpre : coPset → rt_full → iProp Σ) (Cpost : coPset → rt_full → iProp Σ),
+          P lt_cur → P lt_full → P (MagicLty lt_cur lt_full Cpre Cpost)) →
       ∀ lt : lty, P lt.
   Proof.
-    intros P ? ? ? ? ? ? ? ? Hstruct Harr Henum Hopened Hcoreable Hshadow lt.
-    induction lt as [ | | | | | | | | lts IH sls | rt def len lts IH | | | | ] using lty_recursor; [by eauto.. | | | | | | ].
+    intros P ? ? ? ? ? ? ? ? Hstruct Harr Henum Hopened Hcoreable Hshadow Hmagic lt.
+    induction lt as [ | | | | | | | | lts IH sls | rt def len lts IH | | | | | ] using lty_recursor; [by eauto.. | | | | | | | ].
     - eapply Hstruct. intros lt Hin. induction lts as [ | lt' lts IH'].
       + apply elem_of_nil in Hin. done.
       + inversion IH; subst. apply elem_of_cons in Hin as [<- | Hin]; first done.
@@ -953,6 +973,7 @@ Section ltype_def.
     - eapply Hopened; eauto.
     - eapply Hcoreable; eauto.
     - eapply Hshadow; eauto.
+    - eapply Hmagic; eauto.
   Qed.
 
   (** Stronger induction principle for the OpenedLtype case, but requires well-formedness. *)
@@ -977,10 +998,13 @@ Section ltype_def.
       (∀ κs (lt_full : lty), P lt_full → P (CoreableLty κs lt_full)) →
       (∀ (lt_cur : lty) (r_cur : place_rfn (lty_rt lt_cur)) (lt_full : lty),
         P lt_cur → P lt_full → P (ShadowedLty lt_cur r_cur lt_full)) →
+      (∀ (lt_cur lt_full : lty)
+        (Cpre : coPset → lty_rt lt_full → iProp Σ) (Cpost : coPset → lty_rt lt_full → iProp Σ),
+          P lt_cur → P lt_full → P (MagicLty lt_cur lt_full Cpre Cpost)) →
       ∀ lt : lty, lty_wf lt → P lt.
   Proof.
-    intros P ???????? Hstruct Harr Henum Hopened Hcoreable Hshadow lt Hwf.
-    induction lt as [ | | | | | | | | lts IH sls | rt def len lts IH | rt en variant lte IH | rt_inner rt_full lt_cur lt_inner lt_full Cpre Cpost IH1 IH2 IH3 | κ lt_full IH | ] using lty_induction; [by eauto.. | | | | | | ].
+    intros P ???????? Hstruct Harr Henum Hopened Hcoreable Hshadow Hmagic lt Hwf.
+    induction lt as [ | | | | | | | | lts IH sls | rt def len lts IH | rt en variant lte IH | rt_inner rt_full lt_cur lt_inner lt_full Cpre Cpost IH1 IH2 IH3 | κ lt_full IH | | ] using lty_induction; [by eauto.. | | | | | | | ].
     - eapply Hstruct. intros lt Hlt. eapply IH; first done.
       simpl in Hwf. apply Forall_Forall_cb in Hwf.
       eapply Forall_forall; done.
@@ -998,6 +1022,8 @@ Section ltype_def.
     - eapply Hcoreable; eauto.
     - destruct Hwf as (? & ? & <-).
       eapply Hshadow; eauto.
+    - destruct Hwf as (-> & Hcur & Hfull).
+      eapply Hmagic; eauto.
   Qed.
 
   Fixpoint lty_size (lt : lty) : nat :=
@@ -1020,6 +1046,8 @@ Section ltype_def.
         1 + lty_size lt_full
     | ShadowedLty lt_cur r_cur lt_full =>
         1 + lty_size lt_cur + lty_size lt_full
+    | MagicLty lt_cur lt_full Cpre Cpost =>
+        1 + max (lty_size lt_cur) (lty_size lt_full)
     end.
   Definition lty_size_rel : lty → lty → Prop :=
     ltof _ lty_size.
@@ -1065,18 +1093,20 @@ Section ltype_def.
         lty_core lt_full
     | ShadowedLty lt_cur r_cur lt_full =>
         lty_core lt_full
+    | MagicLty lt_cur lt_full Cpre Cpost =>
+        MagicLty lt_cur lt_full Cpre Cpost
     end.
 
   Lemma lty_core_syn_type_eq (lt : lty) :
     lty_st (lty_core lt) = lty_st lt.
   Proof.
-    induction lt as [ | | | | | | | | | ? IH | | | | ]; by eauto.
+    induction lt as [ | | | | | | | | | ? IH | | | | | ]; by eauto.
   Qed.
 
   Lemma lty_core_rt_eq lt :
     lty_rt (lty_core lt) = lty_rt lt.
   Proof.
-    induction lt as [ | | | | ? IH ? | ? IH ? | ? IH | ? ? IH | ? IH ? | ???? IH | | | | ] using lty_induction; simpl; [done.. | | | | | | | | done | done | done].
+    induction lt as [ | | | | ? IH ? | ? IH ? | ? IH | ? ? IH | ? IH ? | ???? IH | | | | | ] using lty_induction; simpl; [done | done | done | done | | | | | | done.. ].
     - by rewrite IH.
     - by rewrite IH.
     - by rewrite IH.
@@ -1085,15 +1115,13 @@ Section ltype_def.
       induction lts as [ | lt lts IH']; first done.
       simpl. rewrite IH; first last. { apply elem_of_cons; eauto. }
       f_equiv. apply IH'. intros. apply IH. apply elem_of_cons; eauto.
-    - done.
-    - done.
   Qed.
 
   (* We cannot get the other direction because of CoreableLty *)
   Lemma lty_core_wf lt :
     lty_wf lt → lty_wf (lty_core lt).
   Proof.
-    induction lt as [ | | | | | | | | lts IH sls | rt def len lts IH | rt en variant lte IH | | rt lt IH | ] using lty_induction; simpl; [done.. | | | | done | | ].
+    induction lt as [ | | | | | | | | lts IH sls | rt def len lts IH | rt en variant lte IH | | rt lt IH | | ] using lty_induction; simpl; [done.. | | | | done | | | ].
     - rewrite -!Forall_Forall_cb.
       rewrite Forall_fmap.
       apply Forall_impl_strong.
@@ -1109,12 +1137,14 @@ Section ltype_def.
       rewrite lty_core_rt_eq. done.
     - done.
     - intros (? & ? & <-). eauto.
+    - intros (? & ?).
+      split; done.
   Qed.
 
   Lemma lty_size_core (lt : lty) :
     lty_size (lty_core lt) ≤ lty_size lt.
   Proof.
-    induction lt as [ | | | | | | | |lts IH sls | rt def len lts IH | | | | ] using lty_induction; simpl; [lia.. | | | lia | lia| lia | lia].
+    induction lt as [ | | | | | | | |lts IH sls | rt def len lts IH | | | | | ] using lty_induction; simpl; [lia.. | | | lia | lia | lia | lia | lia].
     - induction lts as [ | lt lts IH']; simpl; first done.
       efeed pose proof (IH lt) as IH0. { apply elem_of_cons. by left. }
       feed specialize IH'. { intros. apply IH. apply elem_of_cons. by right. }
@@ -1662,7 +1692,14 @@ Section ltype_def.
         ∃ (Heq_cur : rt_cur = lty_rt lt_cur),
         ⌜lty_st lt_cur = lty_st lt_full⌝ ∗
         lty_own_pre core lt_cur k π ((rew Heq_cur in r_cur)) l ∗
-        lty_own_pre core lt_full k π r l)%I
+        lty_own_pre core lt_full k π r l)%I;
+    lty_own_pre core (@MagicLty rt_full lt_cur lt_full Cpre Cpost) k π r l :=
+      (** MagicLty *)
+      match k with (* TODO: MagicType *)
+      | Owned wl => False
+      | Uniq κ γ => False
+      | Shared κ => False
+      end
   .
   Solve Obligations with first [unfold lty_size_rel, ltof; simpl; lia | intros; eauto using struct_lts_size_decreasing, array_lts_size_decreasing].
   Definition lty_own := @lty_own_pre false.
@@ -1688,8 +1725,8 @@ Section ltype_def.
   Lemma lty_core_idemp (lt : lty) :
     lty_core (lty_core lt) = lty_core lt.
   Proof.
-    induction lt as [ | | | | | | | | lts IH ? | rt def len lts IH | | | | ] using lty_induction;
-    [simpl; f_equiv.. | | ]; [solve[eauto].. | | | | | | ].
+    induction lt as [ | | | | | | | | lts IH ? | rt def len lts IH | | | | | ] using lty_induction;
+    [simpl; f_equiv.. | | | ]; [solve[eauto].. | | | | | | | ].
     - done.
     - induction lts as [ | lt lts IH']; first done.
       simpl. rewrite IH; first last. { apply elem_of_cons; eauto. }
@@ -1702,13 +1739,14 @@ Section ltype_def.
     - done.
     - done.
     - done.
+    - done.
   Qed.
 
   Lemma lty_own_has_layout (lt : lty) k π r l :
     lty_own lt k π r l -∗ ∃ ly : layout, ⌜syn_type_has_layout (lty_st lt) ly⌝ ∗ ⌜l `has_layout_loc` ly⌝.
   Proof.
     iIntros "Hown". rewrite /lty_own.
-    iInduction lt as [ | | | | | | | | | rt def len lts IH | | ?? lt_cur lt_inner lt_full Cpre Cpost | | ] "IH" using lty_induction forall (k); simp lty_own_pre.
+    iInduction lt as [ | | | | | | | | | rt def len lts IH | | ?? lt_cur lt_inner lt_full Cpre Cpost | | | ] "IH" using lty_induction forall (k); simp lty_own_pre.
     - iDestruct "Hown" as "(%ly & ? & ? & _)"; eauto.
     - iDestruct "Hown" as "(%ly & ? & ? & _)"; eauto.
     - iDestruct "Hown" as "(%ly & ? & ? & _)"; eauto.
@@ -1732,14 +1770,15 @@ Section ltype_def.
     - iDestruct "Hown" as "(%ly & ? & ? & _)". eauto.
     - iDestruct ("Hown") as (->) "(%Hst & Ha & Hb)".
       simpl. rewrite -Hst. iApply ("IH" with "Ha").
-  Qed.
+    - admit. (* TODO: MagicType *)
+  Admitted.
 
   Lemma lty_own_loc_in_bounds (lt : lty) k π r l ly :
     syn_type_has_layout (lty_st lt) ly →
     lty_own lt k π r l -∗ loc_in_bounds l 0 ly.(ly_size).
   Proof.
     iIntros (Ha) "Hown". rewrite /lty_own.
-    iInduction lt as [ | | | | | | | | | | | ? ??? | | ] "IH" using lty_induction forall (k); simp lty_own_pre.
+    iInduction lt as [ | | | | | | | | | | | ? ??? | | | ] "IH" using lty_induction forall (k); simp lty_own_pre.
     - iDestruct "Hown" as "(%ly' & %Halg' & ? & ? & ? & _)".
       have ?: ly' = ly by eapply syn_type_has_layout_inj. by subst.
     - iDestruct "Hown" as "(%ly' & % & _ & _ & ? & _)".
@@ -1777,15 +1816,19 @@ Section ltype_def.
     - iDestruct "Hown" as (->) "(%Hst & Ha & Hb)".
       simpl in Ha. rewrite -Hst in Ha.
       iApply "IH"; done.
-  Qed.
+    - admit. (* TODO: MagicType *)
+  Admitted.
 
   Lemma lty_own_Owned_true_false (lt : lty) π r l :
-    (match lt with | OpenedLty _ _ _ _ _ | CoreableLty _ _ | ShadowedLty _ _ _ => False | _ => True end) →
+    match lt with
+    | OpenedLty _ _ _ _ _ | CoreableLty _ _ | ShadowedLty _ _ _ | MagicLty _ _ _ _ => False
+    | _ => True
+    end →
     lty_own lt (Owned true) π r l -∗
     have_creds ∗ ▷ lty_own lt (Owned false) π r l.
   Proof.
     iIntros (?) "Hown". rewrite /lty_own.
-    destruct lt as [ | | | | | | | | | | | ? ??? | | ]; simp lty_own_pre.
+    destruct lt as [ | | | | | | | | | | | ? ??? | | | ]; simp lty_own_pre.
     - iDestruct "Hown" as "(%ly & ? & ? & ? & ? & ? & Hcred)". eauto with iFrame.
     - iDestruct "Hown" as "(%ly & ? & ? & ? & ? & % & ? & ? & ? & Hcred)". eauto 8 with iFrame.
     - iDestruct "Hown" as "(%ly & ? & ? & ? & ? & Hcred & % & ? & Hl)". eauto 8 with iFrame.
@@ -1802,15 +1845,19 @@ Section ltype_def.
     - (* this will definitely be a problem also for the other property, because we need two sets of credits
         Maybe change the interpretation to have Owned false for the shadow, always? *)
       done.
+    - done.
   Qed.
   Lemma lty_own_Owned_false_true (lt : lty) π r l :
-    (match lt with | OpenedLty _ _ _ _ _ | CoreableLty _ _ | ShadowedLty _ _ _ => False | _ => True end) →
+    match lt with
+    | OpenedLty _ _ _ _ _ | CoreableLty _ _ | ShadowedLty _ _ _ | MagicLty _ _ _ _ => False
+    | _ => True
+    end →
     (lty_own lt (Owned false) π r l) -∗
     have_creds -∗
     lty_own lt (Owned true) π r l.
   Proof.
     iIntros (?) "Hown Hcred". rewrite /lty_own.
-    destruct lt as [ | | | | | | | | | | | ? ??? | | ]; simp lty_own_pre.
+    destruct lt as [ | | | | | | | | | | | ? ??? | | | ]; simp lty_own_pre.
     - iDestruct "Hown" as "(%ly & ? & ? & ? & ? & ? & _)". iExists _. eauto with iFrame.
     - iDestruct "Hown" as "(%ly & ? & ? & ? & ? & % & ? & ? & ? & _)". iExists _. eauto 8 with iFrame.
     - iDestruct "Hown" as "(%ly & ? & ? & ? & ? & _ & % & ? & Hl)". iExists _. eauto 8 with iFrame.
@@ -1827,6 +1874,7 @@ Section ltype_def.
     - (* this will definitely be a problem also for the other property, because we need two sets of credits
         Maybe change the interpretation to have Owned false for the shadow, always? *)
       done.
+    - done.
   Qed.
 
   Import EqNotations.
@@ -1945,7 +1993,7 @@ Section ltype_def.
     lty_own_pre true (lty_core lt) k π r l ≡ lty_own_pre true lt k π r' l.
   Proof.
     intros ->. rewrite /lty_own_core.
-    induction lt as [ | | | | lt IH κ | lt IH κ | lt IH | lt ls IH | lts IH sls | rt def len lts IH | rt en variant lt IH | | | ] using lty_induction in k, π, r, l, Heq |-*; simpl in *.
+    induction lt as [ | | | | lt IH κ | lt IH κ | lt IH | lt ls IH | lts IH sls | rt def len lts IH | rt en variant lt IH | | | | ] using lty_induction in k, π, r, l, Heq |-*; simpl in *.
     - simp lty_own_pre. rewrite (UIP_refl _ _ Heq). done.
     - simp lty_own_pre. rewrite (UIP_refl _ _ Heq). done.
     - rewrite (UIP_refl _ _ Heq). done.
@@ -2077,6 +2125,7 @@ Section ltype_def.
     - simp lty_own_pre. rewrite (UIP_refl _ _ Heq). done.
     - simp lty_own_pre.
     - simp lty_own_pre.
+    - simp lty_own_pre. done.
   Qed.
   Lemma lty_own_core_core' (lt : lty) k π r Heq l :
     lty_own_pre true (lty_core lt) k π r l ≡ lty_own_pre true lt k π (transport_rfn Heq r) l.
@@ -2155,7 +2204,7 @@ Section ltype_def.
     lty_own_pre true lt k π r l ≡ lty_own_pre core (lty_core lt) k π (transport_rfn Heq r) l.
   Proof.
     rewrite /lty_own_core /lty_own.
-    induction lt as [ | | | | lt IH κ | lt IH κ | lt IH | lt ls IH | lts IH sls | def len lts IH IH' | rt en variant lt  IH | | | ] using lty_induction in k, π, r, l, Heq, core |-*; simpl in *.
+    induction lt as [ | | | | lt IH κ | lt IH κ | lt IH | lt ls IH | lts IH sls | def len lts IH IH' | rt en variant lt  IH | | | | ] using lty_induction in k, π, r, l, Heq, core |-*; simpl in *.
     - simp lty_own_pre. rewrite (UIP_refl _ _ Heq). done.
     - simp lty_own_pre. rewrite (UIP_refl _ _ Heq). done.
     - rewrite (UIP_refl _ _ Heq). simp lty_own_pre. done.
@@ -2285,6 +2334,7 @@ Section ltype_def.
     - rewrite (UIP_refl _ _ Heq). simp lty_own_pre. done.
     - simp lty_own_pre.
     - simp lty_own_pre.
+    - simp lty_own_pre. done.
   Qed.
 
   Local Lemma place_rfn_interp_shared_transport_eq {rt rt'} (r : place_rfn rt) (r' : rt) (Heq : rt = rt') :
@@ -2308,7 +2358,7 @@ Section ltype_def.
     lty_own lt (Shared κ0) π r l -∗ lty_own (lty_core lt) (Shared κ0) π (transport_rfn Heq r) l.
   Proof.
     rewrite /lty_own_core /lty_own.
-    induction lt as [ | | | | lt IH κ | lt IH κ | lt IH | lt ls IH | lts IH sls | rt def len lts IH  | rt en variant lt IH | | | ???? IH1 IH2] using lty_induction in κ0, π, r, l, Heq |-*; simpl in *.
+    induction lt as [ | | | | lt IH κ | lt IH κ | lt IH | lt ls IH | lts IH sls | rt def len lts IH  | rt en variant lt IH | | | ???? IH1 IH2 | ] using lty_induction in κ0, π, r, l, Heq |-*; simpl in *.
     - simp lty_own_pre. iIntros "(% & _ & _ & _ & _ & [])".
     - simp lty_own_pre. iIntros "(% & _ & _ & _ & _ & % & _ & [])".
     - rewrite (UIP_refl _ _ Heq). auto.
@@ -2432,6 +2482,7 @@ Section ltype_def.
     - simp lty_own_pre.
       iIntros "(%Heq_cur & %Hst & Ha & Hb)".
       iApply (IH2 with "Hb").
+    - simp lty_own_pre. iIntros "$".
   Qed.
   (* NOTE: The reverse does not hold because the core of [BlockedLty] is [OfTy], which has a sharing predicate, but [BlockedLty] doesn't *)
 
@@ -2620,6 +2671,21 @@ Section ltype_def.
   Global Arguments ShadowedLtype : simpl never.
   Global Typeclasses Opaque ShadowedLtype.
 
+  Program Definition MagicLtype {rt_cur rt_full} (lt_cur : ltype rt_cur) (lt_full : ltype rt_full)
+      (Cpre : coPset → rt_full → iProp Σ) (Cpost : coPset → rt_full → iProp Σ) : ltype rt_cur := {|
+    ltype_lty := MagicLty (ltype_lty lt_cur) (ltype_lty lt_full) Cpre Cpost;
+  |}.
+  Next Obligation.
+    intros rt_full lt_cur lt_full Cpre Cpost. simpl.
+    rewrite ltype_rt_agree; done.
+  Qed.
+  Next Obligation.
+    intros rt_cur rt_full [lt_cur <- Hcur] [lt_full <- Hfull] Cpre Cpost; simpl.
+    eauto.
+  Qed.
+  Global Typeclasses Opaque MagicLtype.
+  Global Arguments MagicLtype : simpl never.
+
   Import EqNotations.
   Definition ltype_own_pre (core : bool) {rt} (lt : ltype rt) : bor_kind → thread_id → place_rfn rt → loc → iProp Σ :=
     λ k π r l, lty_own_pre core lt.(ltype_lty) k π (rew <- lt.(ltype_rt_agree) in r) l.
@@ -2734,9 +2800,13 @@ Section ltype_def.
       (∀ (rt_full : Type) κs (lt_full : ltype rt_full), P _ lt_full → P _ (CoreableLtype κs lt_full)) →
       (∀ (rt_cur rt_full : Type) (lt_cur : ltype rt_cur) (r_cur : place_rfn rt_cur) (lt_full : ltype rt_full),
         P _ lt_cur → P _ lt_full → P _ (ShadowedLtype lt_cur r_cur lt_full)) →
+      (∀ (rt_cur rt_full : Type) (lt_cur : ltype rt_cur) (lt_full : ltype rt_full)
+        (Cpre : coPset → rt_full → iProp Σ) (Cpost : coPset → rt_full → iProp Σ),
+        P _ lt_cur → P _ lt_full →
+        P _ (MagicLtype lt_cur lt_full Cpre Cpost)) →
       ∀ (rt : Type) (lt : ltype rt), P _ lt.
     Proof.
-      intros Hblocked Hshrblocked Hofty Halias Hmut Hshr Hbox Hptr Hstruct Harr Hen Hopened Hcoreable Hshadow.
+      intros Hblocked Hshrblocked Hofty Halias Hmut Hshr Hbox Hptr Hstruct Harr Hen Hopened Hcoreable Hshadow Hmagic.
 
       assert (P_irrel:
         ∀ rt (lt : lty) Heq1 Heq2 Hwf1 Hwf2, P rt (mk_ltype rt lt Heq1 Hwf1) → P rt (mk_ltype rt lt Heq2 Hwf2)).
@@ -2744,7 +2814,7 @@ Section ltype_def.
         intros Hwf1 Hwf2. rewrite (proof_irrelevance _ Hwf1 Hwf2). done. }
 
       intros rt [lt <- Hwf].
-      induction lt as [ | | | | lt IH κ | lt IH κ | lt IH | lt ls IH | lts IH sls | rt def len lts IH | rt en variant lte IH | rt_inner rt_full lt_cur lt_inner lt_full Cpre Cpost IH_cur IH_inner IH_full | κ lt_full IH | rt_cur lt_cur r_cur lt_full IH_cur IH_full] using lty_induction; simpl.
+      induction lt as [ | | | | lt IH κ | lt IH κ | lt IH | lt ls IH | lts IH sls | rt def len lts IH | rt en variant lte IH | rt_inner rt_full lt_cur lt_inner lt_full Cpre Cpost IH_cur IH_inner IH_full | κ lt_full IH | rt_cur lt_cur r_cur lt_full IH_cur IH_full | rt_full lt_cur lt_full Cpre Cpost IH_cur IH_full ] using lty_induction; simpl.
       - eapply P_irrel. apply Hblocked.
       - eapply P_irrel. apply Hshrblocked.
       - eapply P_irrel. apply Hofty.
@@ -2789,6 +2859,9 @@ Section ltype_def.
       - destruct Hwf as (Hwf_cur & Hwf_full & <-).
         specialize (Hshadow _ _ _ r_cur _ (IH_cur Hwf_cur) (IH_full Hwf_full)).
         eapply P_irrel. eapply Hshadow.
+      - destruct Hwf as (Heq & Hwf_cur & Hwf_full); subst.
+        specialize (Hmagic _ _ _ _ Cpre Cpost (IH_cur Hwf_cur) (IH_full Hwf_full)).
+        eapply P_irrel. eapply Hmagic.
     Qed.
   End induction.
 
@@ -3150,6 +3223,18 @@ Section ltype_def.
     ⌜ltype_st lt_cur = ltype_st lt_full⌝ ∗
     rec _ lt_cur k π (r_cur) l ∗
     rec _ lt_full k π r l.
+
+  Definition magic_ltype_own
+      (rec : ltype_own_type) (rec_core : ltype_own_type)
+      {rt_cur rt_full : Type}
+      (lt_cur : ltype rt_cur) (lt_full : ltype rt_full)
+      (Cpre : coPset → rt_full → iProp Σ) (Cpost : coPset → rt_full → iProp Σ)
+      (k : bor_kind) (π : thread_id) (r : place_rfn rt_cur) (l : loc) : iProp Σ :=
+    match k with (* TODO: MagicType *)
+    | Owned wl => False
+    | Uniq κ γ => False
+    | Shared κ => False
+    end.
 
   Lemma ltype_own_pre_ofty_unfold {rt} (ty : type rt) (core : bool) k π r l :
     ltype_own_pre core (OfTy ty) k π r l ≡ lty_of_ty_own ty k π r l.
@@ -3679,6 +3764,23 @@ Section ltype_def.
     intros ?. done.
   Qed.
 
+  Lemma ltype_own_magic_unfold {rt_cur rt_full : Type} (lt_cur : ltype rt_cur) (lt_full : ltype rt_full)
+      (Cpre : coPset → rt_full → iProp Σ) (Cpost : coPset → rt_full → iProp Σ) k π r l :
+    ltype_own (MagicLtype lt_cur lt_full Cpre Cpost) k π r l ≡ magic_ltype_own (@ltype_own) (@ltype_own_core) lt_cur lt_full Cpre Cpost k π r l.
+  Proof.
+    rewrite /magic_ltype_own ?ltype_own_core_unseal /ltype_own_core_def ?ltype_own_unseal /ltype_own_def /ltype_own_pre.
+    simp lty_own_pre.
+    done.
+  Qed.
+  Lemma ltype_own_core_magic_unfold {rt_cur rt_full : Type} (lt_cur : ltype rt_cur) (lt_full : ltype rt_full)
+      (Cpre : coPset → rt_full → iProp Σ) (Cpost : coPset → rt_full → iProp Σ) k π r l :
+    ltype_own_core (MagicLtype lt_cur lt_full Cpre Cpost) k π r l ≡ magic_ltype_own (@ltype_own) (@ltype_own_core) lt_cur lt_full Cpre Cpost k π r l.
+  Proof.
+    rewrite -ltype_own_magic_unfold.
+    rewrite ltype_own_core_unseal ltype_own_unseal /ltype_own_core_def /ltype_own_def /ltype_own_pre.
+    simp lty_own_pre. done.
+  Qed.
+
   (** Lifting basic lemmas to [ltype] *)
 
   (* NOTE: This does not hold true for [OpenedLtype]! *)
@@ -3777,7 +3879,10 @@ Section ltype_def.
   Qed.
 
   Lemma ltype_own_Owned_true_false {rt} (lt : ltype rt) π r l :
-    match ltype_lty lt with | OpenedLty _ _ _ _ _ | CoreableLty _ _ | ShadowedLty _ _ _ => False | _ => True end →
+    match ltype_lty lt with
+    | OpenedLty _ _ _ _ _ | CoreableLty _ _ | ShadowedLty _ _ _ | MagicLty _ _ _ _ => False
+    | _ => True
+    end →
     ltype_own lt (Owned true) π r l -∗
     have_creds ∗ ▷ ltype_own lt (Owned false) π r l.
   Proof.
@@ -3786,7 +3891,10 @@ Section ltype_def.
     apply lty_own_Owned_true_false.
   Qed.
   Lemma ltype_own_Owned_false_true {rt} (lt : ltype rt) π r l :
-    match ltype_lty lt with | OpenedLty _ _ _ _ _ | CoreableLty _ _ | ShadowedLty _ _ _ => False | _ => True end →
+    match ltype_lty lt with
+    | OpenedLty _ _ _ _ _ | CoreableLty _ _ | ShadowedLty _ _ _ | MagicLty _ _ _ _ => False
+    | _ => True
+    end →
     ltype_own lt (Owned false) π r l -∗
     have_creds -∗
     ltype_own lt (Owned true) π r l.
@@ -3936,6 +4044,14 @@ Section ltype_def.
     - apply UIP_t.
     - apply proof_irrelevance.
   Qed.
+  Lemma ltype_core_magic {rt_cur rt_full} (lt_cur : ltype rt_cur) (lt_full : ltype rt_full) Cpre Cpost :
+    ltype_core (MagicLtype lt_cur lt_full Cpre Cpost) = MagicLtype lt_cur lt_full Cpre Cpost.
+  Proof.
+    rewrite /ltype_core /MagicLtype /=.
+    f_equiv; simpl.
+    - apply UIP_t.
+    - apply proof_irrelevance.
+  Qed.
   Lemma ltype_core_uninit st :
     ltype_core (UninitLtype st) = UninitLtype st.
   Proof.
@@ -3984,6 +4100,9 @@ Section ltype_def.
   Proof. done. Qed.
   Lemma ltype_st_shadowed {rt_cur rt_full} (lt_cur : ltype rt_cur) (r_cur : place_rfn rt_cur) (lt_full : ltype rt_full) :
     ltype_st (ShadowedLtype lt_cur r_cur lt_full) = ltype_st lt_full.
+  Proof. done. Qed.
+  Lemma ltype_st_magic {rt_cur rt_full} (lt_cur : ltype rt_cur) (lt_full : ltype rt_full) Cpre Cpost :
+    ltype_st (MagicLtype lt_cur lt_full Cpre Cpost) = ltype_st lt_cur.
   Proof. done. Qed.
 
   (** Lifting the core equations to ltypes *)
@@ -4036,6 +4155,7 @@ Section ltype_def.
     | OpenedLty _ _ _ _ _  => []
     | CoreableLty κs _ => κs
     | ShadowedLty lt_cur r_cur lt_full => lty_blocked_lfts lt_full
+    | MagicLty _ _ _ _ => []
     end.
 
   Definition ltype_blocked_lfts {rt} (lt : ltype rt) : list lft :=
@@ -4064,6 +4184,7 @@ Section ltype_def.
     | CoreableLty _ _ => True
     | ShadowedLty lt _ _ =>
         False
+    | MagicLty _ _ _ _ => False
     end.
   Definition ltype_uniq_deinitializable {rt} (lt : ltype rt) :=
     lty_uniq_deinitializable lt.(ltype_lty).
@@ -4128,6 +4249,7 @@ Section ltype_def.
     | CoreableLty _ _ => Some None
     | ShadowedLty lt _ _ =>
         None
+    | MagicLty _ _ _ _ => None
     end.
   Definition ltype_uniq_extractable {rt} (lt : ltype rt) : option (option lft) :=
     lty_uniq_extractable lt.(ltype_lty).
@@ -4236,6 +4358,8 @@ Ltac simp_ltype_core Heq :=
       rewrite (ltype_core_coreable) in Heq
   | _ = ltype_core (ShadowedLtype _ _ _) =>
       rewrite (ltype_core_shadowed _ _ _) in Heq
+  | _ = ltype_core (MagicLtype _ _ _ _ _) =>
+      rewrite (ltype_core_magic) in Heq
   end.
 Ltac simp_ltype_st Heq :=
   cbn in Heq;
@@ -4268,6 +4392,8 @@ Ltac simp_ltype_st Heq :=
       rewrite (ltype_st_coreable) in Heq
   | _ = ltype_st (ShadowedLtype _ _ _) =>
       rewrite (ltype_st_shadowed _ _ _) in Heq
+  | _ = ltype_st (MagicLtype _ _ _ _ _) =>
+      rewrite (ltype_st_magic) in Heq
   end.
 
 Ltac simp_ltype :=
@@ -5390,6 +5516,14 @@ Section blocked.
       rewrite -ltype_own_core_equiv. iApply ("Ha2" with "Hdead Hb").
   Qed.
 
+  Lemma magic_ltype_imp_unblockable {rt_cur rt_full} (lt_cur : ltype rt_cur) (lt_full : ltype rt_full) Cpre Cpost κs :
+    ⊢ imp_unblockable κs (MagicLtype lt_cur lt_full Cpre Cpost).
+  Proof.
+    iModIntro. iSplitL.
+    - iIntros (κ' ????). rewrite ltype_own_core_equiv ltype_core_magic. eauto.
+    - iIntros (????). rewrite ltype_own_core_equiv ltype_core_magic. eauto.
+  Qed.
+
   (** Once all the blocked lifetimes are dead, every ltype is unblockable to its core. *)
   Lemma imp_unblockable_blocked_dead {rt} (lt : ltype rt) :
     ⊢ imp_unblockable (ltype_blocked_lfts lt) lt.
@@ -5440,6 +5574,8 @@ Section blocked.
     - iIntros (rt_full κ' lt_full Hdead). iApply coreable_ltype_imp_unblockable.
     - iIntros (rt_cur rt_full lt_cur r_cur lt_full _ Hub).
       iApply shadowed_ltype_imp_unblockable. done.
+    - iIntros (rt_cur rt_full lt_cur lt_full Cpre Cpost IH1 IH2).
+      iApply magic_ltype_imp_unblockable.
   Qed.
 
   (** We can essentiallly rewrite with [ltype_eq] when proving [imp_unblockable]. *)
